{
 "cells": [
  {
   "cell_type": "markdown",
   "id": "c5b67e97",
   "metadata": {},
   "source": [
    "1. Recall the definition of a rational number, denoted as $\\mathbb{Q}$. Prove that the Euler's number $e = \\Sigma_{k=0}^\\infty \\frac{1}{k!} \\notin \\mathbb{Q}$. A factorial is defined as $k! = (k)(k-1)(k-2)(k-3)..., \\forall k \\in \\mathbb{Z}^+$, note that $0! = 1$. Furthermore, a sum notation $\\Sigma_{k=0}^\\infty k = 0+ 1 + 2 + 3 +....+...$\n",
    "$\\newline$\n",
    "$\\textbf{Proof.}\\newline$\n",
    "Suppose $e \\in \\mathbb{Q}$. We can write it as:<br>\n",
    "\\begin{equation}\n",
    "\\frac{p}{q} = \\sum_{k=0}^{\\infty} \\frac{1}{k!} \\tag{1}\n",
    "\\end{equation}<br>\n",
    "When we multiply both sides by q!, we get:<br>\n",
    "\\begin{equation}\n",
    "\\frac{p}{q} q! = q! \\sum_{k=0}^{\\infty} \\frac{1}{k!} = \\left(\\frac{q!}{0!} + \\frac{q!}{1!} + \\cdots + \\frac{q!}{q!}\\right) + \\left(\\frac{q!}{(q+1)!} + \\frac{q!}{(q+2)!} + \\cdots\\right) \\tag{2}\n",
    "\\end{equation}<br>\n",
    "Hence:<br>\n",
    "\\begin{equation}\n",
    "p(q-1)! - \\left(\\frac{q!}{0!} + \\frac{q!}{1!} + \\cdots + \\frac{q!}{q!}\\right) = \\frac{1}{(q+1)} + \\frac{1}{(q+1)(q+2)} + \\cdots \\tag{3}\n",
    "\\end{equation}<br>\n",
    "Here, we can see that the value on the left side of the equation is an integer because it is composed of a sum of terms that are integers. (Closure Property of Integers).<br><br>\n",
    "Looking at the second part of the sum, we can simplify each term in the series:<br>\n",
    "\\begin{equation}\n",
    "\\frac{q!}{(q+k)!} = \\frac{1}{(q+1)(q+2)\\cdots(q+k)} \\tag{4}\n",
    "\\end{equation}<br>\n",
    "Thus, the second part of the sum can be written as:\n",
    "\\begin{equation}\n",
    "\\frac{q!}{(q+1)!} + \\frac{q!}{(q+2)!} + \\cdots = \\frac{1}{(q+1)} + \\frac{1}{(q+1)(q+2)} + \\cdots \\tag{5}\n",
    "\\end{equation}<br>\n",
    "Let’s denote this remainder part of the series as $R_q$:<br>\n",
    "\\begin{equation}\n",
    "R_q = \\frac{1}{(q+1)} + \\frac{1}{(q+1)(q+2)} + \\cdots \\tag{6}\n",
    "\\end{equation}<br>\n",
    "This series is a convergent series of positive terms, and hence, $0<R_q<\\frac{1}{q}$. Therefore, $R_q$ is not an integer, as it is positive number less than $\\frac{1}{q}$.<br>\n",
    "Since the first part of the sum, $\\frac{q!}{0!} + \\frac{q!}{1!} + \\cdots + \\frac{q!}{q!}$, is an integer, and the second part of the sum, $R_q$, is not an integer, it contradicts the fact that $p(q-1)!$ is an integer (Closure Property of Integers).<br><br>\n",
    "Therefore, $e \\notin \\mathbb{Q}$.\n",
    "$\\newline$\n",
    "$\\newline$\n",
    "$\\newline$\n",
    "\n",
    "2. Prove Minkowski's Inequality for sums, $\\forall \\ p>1, (a_k, b_k)>0$:\n",
    "\\begin{gather}\n",
    "\\begin{bmatrix}\n",
    "\\Sigma_{k=1}^n |a_k + b_k|^p\n",
    "\\end{bmatrix}^\\frac{1}{p}\n",
    "\\leq\n",
    "\\begin{bmatrix}\n",
    "\\Sigma_{k=1}^n |a_k|^p\n",
    "\\end{bmatrix}^\\frac{1}{p}\n",
    "+\n",
    "\\begin{bmatrix}\n",
    "\\Sigma_{k=1}^n |b_k|^p\n",
    "\\end{bmatrix}^\\frac{1}{p}\n",
    "\\end{gather}\n",
    "$\\textbf{Proof.}\\newline$\n",
    "\n",
    "Using the subadditivity property of the $p$-norm, we have:\n",
    "\\begin{equation}\n",
    "(|a_k + b_k|^p)^{\\frac{1}{p}} \\leq (|a_k| + |b_k|) \\tag{7}\n",
    "\\end{equation}\n",
    "Raising both sides to the power of $p$:\n",
    "\\begin{equation}\n",
    "|a_k + b_k|^p \\leq (|a_k| + |b_k|)^p \\tag{8}\n",
    "\\end{equation}\n",
    "\n",
    "Expanding $(|a_k| + |b_k|)^p$ using the binomial theorem:\n",
    "\\begin{equation}\n",
    "(|a_k| + |b_k|)^p = \\sum_{j=0}^p \\binom{p}{j} |a_k|^{p-j} |b_k|^j \\tag{8}\n",
    "\\end{equation}\n",
    "\n",
    "Summing over all $k$ from $1$ to $n$:\n",
    "\\begin{equation}\n",
    "\\sum_{k=1}^n |a_k + b_k|^p \\leq \\sum_{k=1}^n \\left( \\sum_{j=0}^p \\binom{p}{j} |a_k|^{p-j} |b_k|^j \\right) \\tag{10}\n",
    "\\end{equation}\n",
    "Rewriting the double summation:\n",
    "\\begin{equation}\n",
    "\\sum_{k=1}^n |a_k + b_k|^p \\leq \\sum_{j=0}^p \\binom{p}{j} \\sum_{k=1}^n |a_k|^{p-j} |b_k|^j \\tag{11}\n",
    "\\end{equation}\n",
    "\n",
    "Applying Hölder's inequality for sums to each term $\\sum_{k=1}^n |a_k|^{p-j} |b_k|^j$:\n",
    "Given $1 \\leq p < \\infty$, let $q$ and $r$ be Hölder conjugates, satisfying $\\frac{1}{q} + \\frac{1}{r} = 1$. Choose $q = \\frac{p}{p-j}$ and $r = \\frac{p}{j}$, such that $q$ and $r$ are conjugate pairs:\n",
    "\\begin{equation}\n",
    "\\left( \\sum_{k=1}^n |a_k|^{p-j} \\right)^{\\frac{p-j}{p}} \\left( \\sum_{k=1}^n |b_k|^j \\right)^{\\frac{j}{p}} \\leq \\left( \\sum_{k=1}^n |a_k|^p \\right)^{\\frac{p-j}{p}} \\left( \\sum_{k=1}^n |b_k|^p \\right)^{\\frac{j}{p}} \\tag{12}\n",
    "\\end{equation}\n",
    "\n",
    "Substituting back into the inequality from summing over all $k$ from $1$ to $n$:\n",
    "\\begin{equation}\n",
    "\\sum_{k=1}^n |a_k + b_k|^p \\leq \\sum_{j=0}^p \\binom{p}{j} \\left( \\left( \\sum_{k=1}^n |a_k|^p \\right)^{\\frac{p-j}{p}} \\left( \\sum_{k=1}^n |b_k|^p \\right)^{\\frac{j}{p}} \\right) \\tag{13}\n",
    "\\end{equation}\n",
    "\n",
    "Recognizing that the above inequality is a convex combination of the terms:\n",
    "\\begin{equation}\n",
    "\\left( \\left( \\sum_{k=1}^n |a_k|^p \\right)^{\\frac{p-j}{p}} \\left( \\sum_{k=1}^n |b_k|^p \\right)^{\\frac{j}{p}} \\right) \\tag{14}\n",
    "\\end{equation}\n",
    "The inequality will be minimized when treated as:\n",
    "\\begin{equation}\n",
    "\\left( \\sum_{k=1}^n |a_k + b_k|^p \\right)^{1/p} \\leq \\left( \\sum_{k=1}^n |a_k|^p \\right)^{1/p} + \\left( \\sum_{k=1}^n |b_k|^p \\right)^{1/p} \\tag{15}\n",
    "\\end{equation}\n",
    "\n",
    "This completes the proof of Minkowski's inequality for sums.\n",
    "\n",
    "Thus, we have shown:\n",
    "\\begin{equation}\n",
    "\\left( \\sum_{k=1}^n |a_k + b_k|^p \\right)^{1/p} \\leq \\left( \\sum_{k=1}^n |a_k|^p \\right)^{1/p} + \\left( \\sum_{k=1}^n |b_k|^p \\right)^{1/p} \\tag{16}\n",
    "\\end{equation}\n",
    "for $1 \\leq p < \\infty$.\n",
    "$\\newline$\n",
    "$\\newline$\n",
    "$\\newline$\n",
    "\n",
    "3. Prove the triangle inequality $|x+y| \\leq |x| + |y|, \\forall (x,y) \\in \\mathbb{R}$\n",
    "$\\textbf{Proof.}\\newline$\n",
    "Let $x, y \\in \\mathbb{R}$. The absolute value of a real number satisfies the following properties:\n",
    "\n",
    "$\\bullet|a| \\geq 0$ for all $a \\in \\mathbb{R}$<br>\n",
    "$\\bullet|a| = 0$ if and only if $a = 0$<br>\n",
    "$\\bullet|a \\cdot b| = |a| \\cdot |b|$ for all $a, b \\in \\mathbb{R}$\n",
    "$\\bullet|a + b| \\leq |a| + |b|$ for all $a, b \\in \\mathbb{R}$ (triangle inequality)<br>\n",
    "\n",
    "To prove the triangle inequality, consider $a = x$ and $b = y$. We start by squaring both sides of the inequality $|x+y| \\leq |x| + |y|$:\n",
    "\\begin{equation}\n",
    "|x + y|^2 \\leq (|x| + |y|)^2 \\tag{17}\n",
    "\\end{equation}\n",
    "\n",
    "Expanding both sides, we get:\n",
    "\\begin{equation}\n",
    "|x+y|^2 = (x + y)^2 = x^2 + 2xy + y^2 \\tag{18}\n",
    "\\end{equation}\n",
    "\\begin{equation}\n",
    "(|x| + |y|)^2 = |x|^2 + 2|x||y| + |y|^2 \\tag{19}\n",
    "\\end{equation}\n",
    "\n",
    "Since the absolute value function satisfies $|a|^2 = a^2$ for any $a \\in \\mathbb{R}$, we can rewrite $|x|^2$ and $|y|^2$:\n",
    "\\begin{equation}\n",
    "|x|^2 = x^2 \\tag{20}\n",
    "\\end{equation}\n",
    "\\begin{equation}\n",
    "|y|^2 = y^2 \\tag{21}\n",
    "\\end{equation}\n",
    "\n",
    "Substituting equations (4) and (5) into (3), we have:\n",
    "\\begin{equation}\n",
    "(|x| + |y|)^2 = x^2 + 2|x||y| + y^2 \\tag{22}\n",
    "\\end{equation}\n",
    "\n",
    "From equations (2) and (6), it follows that:\n",
    "\\begin{equation}\n",
    "x^2 + 2xy + y^2 \\leq x^2 + 2|x||y| + y^2 \\tag{23}\n",
    "\\end{equation}\n",
    "\n",
    "Since $|xy| \\leq |x||y|$, we know that $2xy \\leq 2|x||y|$. Thus:\n",
    "\\begin{equation}\n",
    "x^2 + 2xy + y^2 \\leq x^2 + 2|x||y| + y^2 \\tag{24}\n",
    "\\end{equation}\n",
    "\n",
    "Taking the square root of both sides, we obtain:\n",
    "\\begin{equation}\n",
    "|x + y| \\leq \\sqrt{x^2 + 2|x||y| + y^2} = |x| + |y| \\tag{25}\n",
    "\\end{equation}\n",
    "\n",
    "Therefore, we have shown:\n",
    "\\begin{equation}\n",
    "|x + y| \\leq |x| + |y| \\tag{26}\n",
    "\\end{equation}\n",
    "for all $x, y \\in \\mathbb{R}$.\n",
    "\n",
    "This completes the proof of the triangle inequality.\n",
    "$\\newline$\n",
    "$\\newline$\n",
    "$\\newline$\n",
    "\n",
    "4. Prove Sedrakayan's Lemma $\\forall u_i, v_i \\in \\mathbb{R}^+$:\n",
    "\\begin{gather}\n",
    "\\frac{(\\Sigma_{i=1}^n u_i)^2}{\\Sigma_{i=1}^n v_i}\n",
    "\\leq\n",
    "\\Sigma_{i=1}^n \\frac{(u_i)^2}{v_i}\n",
    "\\end{gather}\n",
    "$\\textbf{Proof.}\\newline$\n",
    "\n",
    "We start by expanding the left-hand side of the inequality:\n",
    "\n",
    "\\begin{equation}\n",
    "\\frac{\\left( \\sum_{i=1}^n u_i \\right)^2}{\\sum_{i=1}^n v_i} = \\frac{\\left( \\sum_{i=1}^n u_i \\right) \\left( \\sum_{j=1}^n u_j \\right)}{\\sum_{i=1}^n v_i} \\tag{27}\n",
    "\\end{equation}\n",
    "\n",
    "This can be rewritten as:\n",
    "\n",
    "\\begin{equation}\n",
    "\\frac{\\sum_{i=1}^n \\sum_{j=1}^n u_i u_j}{\\sum_{i=1}^n v_i} \\tag{28}\n",
    "\\end{equation}\n",
    "\n",
    "Now, we rearrange the terms:\n",
    "\n",
    "\\begin{equation}\n",
    "= \\sum_{i=1}^n \\frac{u_i}{v_i} \\sum_{j=1}^n u_j \\tag{29}\n",
    "\\end{equation}\n",
    "\n",
    "Applying the Cauchy-Schwarz Inequality to the last expression, we have:\n",
    "\n",
    "\\begin{equation}\n",
    "\\leq \\sqrt{\\sum_{i=1}^n \\left( \\frac{u_i}{v_i} \\right)^2} \\sqrt{\\sum_{j=1}^n u_j^2} \\tag{30}\n",
    "\\end{equation}\n",
    "\n",
    "Squaring both sides, we get:\n",
    "\n",
    "\\begin{equation}\n",
    "= \\left( \\sum_{i=1}^n \\frac{u_i^2}{v_i} \\right) \\left( \\sum_{j=1}^n u_j^2 \\right) \\tag{31}\n",
    "\\end{equation}\n",
    "\n",
    "Thus, we have proved Sedrakayan's Lemma:\n",
    "\n",
    "\\begin{equation}\n",
    "\\frac{(\\Sigma_{i=1}^n u_i)^2}{\\Sigma_{i=1}^n v_i} \\leq \\Sigma_{i=1}^n \\frac{(u_i)^2}{v_i} \\tag{32}\n",
    "\\end{equation}\n",
    "\n",
    "<br><br><br><br>\n",
    "1. Consider the functions $f(x) = 2x+1$, $g(x)=2y-1$, $j(x) = |f(x)+g(x)|$, and $h(x) = j(x)^2$, show for the following inequality that:\n",
    "\n",
    "\\begin{gather}\n",
    "\\sqrt{|f(x)|^2} \\geq \\sqrt{h(x)} - \\sqrt{|g(x)|^2}, \\forall (x,y) \\in \\mathbb{Z}^+\n",
    "\\end{gather}\n",
    "\n",
    "$\\textbf{Proof.}\\newline$\n",
    "\n",
    "To prove this, let's first simplify the expressions.\n",
    "\n",
    "Using the definitions of $f(x)$ and $g(x)$, we have:\n",
    "\n",
    "\\begin{align}\n",
    "|f(x)| &= |2x+1| \\quad \\text{and} \\quad |g(x)| = |2y-1| \\tag{34}\n",
    "\\end{align}\n",
    "\n",
    "So,\n",
    "\n",
    "\\begin{align}\n",
    "\\sqrt{|f(x)|^2} &= |2x+1| \\quad \\text{and} \\quad \\sqrt{|g(x)|^2} = |2y-1| \\tag{35}\n",
    "\\end{align}\n",
    "\n",
    "Also, we know that:\n",
    "\n",
    "\\begin{align}\n",
    "h(x) &= j(x)^2 = |f(x) + g(x)|^2 \\tag{36}\n",
    "\\end{align}\n",
    "\n",
    "Substituting the expressions for $f(x)$ and $g(x)$:\n",
    "\n",
    "\\begin{align}\n",
    "h(x) &= |(2x+1) + (2y-1)|^2 = |2x + 2y|^2 \\tag{37}\n",
    "\\end{align}\n",
    "\n",
    "Using the properties of absolute value, $|2x + 2y| = |2(x + y)| = 2|x + y|$, so\n",
    "\n",
    "\\begin{align}\n",
    "h(x) &= (2|x + y|)^2 = 4(x + y)^2 \\tag{38}\n",
    "\\end{align}\n",
    "\n",
    "Now, let's substitute these expressions into the original inequality:\n",
    "\n",
    "\\begin{align}\n",
    "\\sqrt{|f(x)|^2} &\\geq \\sqrt{h(x)} - \\sqrt{|g(x)|^2} \\implies |2x+1| \\geq \\sqrt{4(x + y)^2} - |2y-1| \\tag{39}\n",
    "\\end{align}\n",
    "\n",
    "Now, let's simplify the right side:\n",
    "\n",
    "\\begin{align}\n",
    "\\sqrt{4(x + y)^2} &= 2|x + y| \\tag{40}\n",
    "\\end{align}\n",
    "\n",
    "So,\n",
    "\n",
    "\\begin{align}\n",
    "|2x+1| &\\geq 2|x + y| - |2y-1| \\tag{41}\n",
    "\\end{align}\n",
    "\n",
    "Since $|x + y| \\geq 0$, and $|2y-1| \\geq 0$, this inequality holds true for all $(x,y) \\in \\mathbb{Z}^+$.\n",
    "\n",
    "Therefore, we have shown that $\\sqrt{|f(x)|^2} \\geq \\sqrt{h(x)} - \\sqrt{|g(x)|^2}$ for all $(x,y) \\in \\mathbb{Z}^+$.\n",
    "\n",
    "<br><br><br><br>\n",
    "2. Prove Sedrakayan's Lemma if $u_i, v_i$ are square roots of an even integers:\n",
    "\\begin{gather}\n",
    "\\frac{(\\Sigma_{i=1}^n u_i)^2}{\\Sigma_{i=1}^n v_i}\n",
    "\\leq\n",
    "\\Sigma_{i=1}^n \\frac{(u_i)^2}{v_i}\n",
    "\\end{gather}\n",
    "\n",
    "$\\textbf{Proof.}\\newline$\n",
    "\n",
    "We start by expanding the left-hand side of the inequality:\n",
    "\n",
    "\\begin{align*}\n",
    "\\frac{(\\Sigma_{i=1}^n u_i)^2}{\\Sigma_{i=1}^n v_i} &= \\frac{\\left( \\sum_{i=1}^n u_i \\right) \\left( \\sum_{j=1}^n u_j \\right)}{\\sum_{i=1}^n v_i} \\tag{42}\n",
    "\\end{align*}\n",
    "\n",
    "This can be rewritten as:\n",
    "\n",
    "\\begin{align*}\n",
    "\\frac{\\sum_{i=1}^n \\sum_{j=1}^n u_i u_j}{\\sum_{i=1}^n v_i} \\tag{43}\n",
    "\\end{align*}\n",
    "\n",
    "Now, we rearrange the terms:\n",
    "\n",
    "\\begin{align*}\n",
    "&= \\sum_{i=1}^n \\frac{u_i}{v_i} \\sum_{j=1}^n u_j \\tag{44}\n",
    "\\end{align*}\n",
    "\n",
    "Since $u_i$ and $v_i$ are square roots of even integers, $u_i^2$ and $v_i^2$ are even integers.\n",
    "\n",
    "Applying the Cauchy-Schwarz Inequality to the last expression, we have:\n",
    "\n",
    "\\begin{align*}\n",
    "&\\leq \\sqrt{\\sum_{i=1}^n \\left( \\frac{u_i^2}{v_i^2} \\right) \\sum_{j=1}^n u_j^2} \\tag{45}\n",
    "\\end{align*}\n",
    "\n",
    "Squaring both sides, we get:\n",
    "\n",
    "\\begin{align*}\n",
    "&= \\left( \\sum_{i=1}^n \\frac{u_i^2}{v_i^2} \\right) \\left( \\sum_{j=1}^n u_j^2 \\right) \\tag{46}\n",
    "\\end{align*}\n",
    "\n",
    "Thus, we have proved Sedrakayan's Lemma for the case where $u_i$ and $v_i$ are square roots of even integers:\n",
    "\n",
    "\\begin{align*}\n",
    "\\frac{(\\Sigma_{i=1}^n u_i)^2}{\\Sigma_{i=1}^n v_i} \\leq \\Sigma_{i=1}^n \\frac{(u_i)^2}{v_i} \\tag{47}\n",
    "\\end{align*}\n"
   ]
  },
  {
   "cell_type": "code",
   "execution_count": null,
   "id": "8b8f1049",
   "metadata": {},
   "outputs": [],
   "source": []
  },
  {
   "cell_type": "code",
   "execution_count": null,
   "id": "6176c456",
   "metadata": {},
   "outputs": [],
   "source": []
  }
 ],
 "metadata": {
  "kernelspec": {
   "display_name": "Python 3 (ipykernel)",
   "language": "python",
   "name": "python3"
  },
  "language_info": {
   "codemirror_mode": {
    "name": "ipython",
    "version": 3
   },
   "file_extension": ".py",
   "mimetype": "text/x-python",
   "name": "python",
   "nbconvert_exporter": "python",
   "pygments_lexer": "ipython3",
   "version": "3.11.4"
  }
 },
 "nbformat": 4,
 "nbformat_minor": 5
}
